CheckRec.lean
@@ -1,0 +1,187 @@
+import Lean
+
+open Lean Meta
+
+def checkRec (iv : InductiveVal) : MetaM Unit := do
+  if iv.isNested then
+    throwError "nested inductives are unsupported"
+
+  let all := iv.all.toArray
+
+  let inducts ← all.mapM fun n => do
+    let iv ← getConstInfoInduct n
+    return (iv, ← iv.ctors.toArray.mapM getConstInfoCtor, ← getConstInfoRec (mkRecName n))
+
+  let levels := iv.levelParams.map .param
+
+  let elim_level :=
+    let (iv, _, rv) := inducts[0]!
+    if rv.levelParams.length > iv.levelParams.length then
+      .param rv.levelParams.head!
+    else
+      .zero
+
+  forallBoundedTelescope iv.type iv.numParams fun params _ => do
+  let motives ← inducts.mapM fun (iv, _) => do
+    forallTelescopeReducing (← instantiateForall iv.type params) fun indices _ =>
+    withLocalDeclD `t (mkAppN (mkAppN (.const iv.name levels) params) indices) fun major => do
+    let motive ← mkForallFVars (indices.push major) <| .sort elim_level
+    return (`motive, fun _ => return motive)
+  withLocalDeclsD motives fun motives => do
+  let minors ← motives.zip inducts |>.concatMapM fun (motive, (_, cvs, _)) => cvs.mapM fun cv => do
+    forallTelescope (← instantiateForall cv.type params) fun fields t => do
+    let ihs ← fields.filterMapM fun field => do
+      forallTelescopeReducing (← inferType field) fun xs t =>
+        t.getAppFn.constName?.bindM fun fn => do
+        all.indexOf? fn |>.mapM fun idx => do
+        let ih ← mkForallFVars xs <| .app (mkAppN motives[idx]! t.getAppArgs[iv.numParams:]) (mkAppN field xs)
+        return (.anonymous, fun _ => return ih)
+    withLocalDeclsD ihs fun ihs => do
+    let minor ← mkForallFVars (fields ++ ihs) <| .app (mkAppN motive t.getAppArgs[iv.numParams:]) (mkAppN (mkAppN (.const cv.name levels) params) fields)
+    return (.anonymous, fun _ => return minor)
+  withLocalDeclsD minors fun minors =>
+  for (motive, iv, _, rv) in motives.zip inducts do
+    forallTelescopeReducing (← instantiateForall iv.type params) fun indices _ =>
+    withLocalDeclD `t (mkAppN (mkAppN (.const iv.name levels) params) indices) fun major => do
+    let type ← mkForallFVars (params ++ motives ++ minors ++ indices |>.push major) <| .app (mkAppN motive indices) major
+
+    let type ← transform type fun e => return .continue e.consumeTypeAnnotations
+    let rvType ← transform rv.type fun e => return .continue e.consumeTypeAnnotations
+    if !type.eqv rvType then
+      logInfo m!"{iv.name}{Format.line}{type}{Format.line}{rvType}"
+
+def checkCasesOn (iv : InductiveVal) : MetaM Unit := do
+  if iv.isNested then
+    throwError "nested inductives are unsupported"
+
+  let all := iv.all.toArray
+
+  let inducts ← all.mapM fun n => do
+    let iv ← getConstInfoInduct n
+    return (iv, ← iv.ctors.toArray.mapM getConstInfoCtor, ← getConstInfoRec (mkRecName n))
+
+  let levels := iv.levelParams.map .param
+
+  let elim_level :=
+    let (iv, _, rv) := inducts[0]!
+    if rv.levelParams.length > iv.levelParams.length then
+      .param rv.levelParams.head!
+    else
+      .zero
+
+  forallBoundedTelescope iv.type iv.numParams fun params _ => do
+  for (iv, cvs, _) in inducts do
+    forallTelescopeReducing (← instantiateForall iv.type params) fun indices _ =>
+    withLocalDeclD `t (mkAppN (mkAppN (.const iv.name levels) params) indices) fun major => do
+    withLocalDeclD `motive (← mkForallFVars (indices.push major) <| .sort elim_level) fun motive => do
+    let minors ← cvs.mapM fun cv => do
+      forallTelescope (← instantiateForall cv.type params) fun fields t => do
+      let minor ← mkForallFVars fields <| .app (mkAppN motive t.getAppArgs[iv.numParams:]) (mkAppN (mkAppN (.const cv.name levels) params) fields)
+      return (.anonymous, fun _ => return minor)
+    withLocalDeclsD minors fun minors => do
+    let type ← mkForallFVars (params ++ #[motive] ++ indices ++ #[major] ++ minors) <| .app (mkAppN motive indices) major
+
+    let type ← transform type fun e => return .continue e.consumeTypeAnnotations
+    let casesOnType ← transform (← getConstInfo (mkCasesOnName iv.name)).type fun e => return .continue e.consumeTypeAnnotations
+    if !type.eqv casesOnType then
+      logInfo m!"{iv.name}{Format.line}{type}{Format.line}{casesOnType}"
+
+run_elab
+  (← getEnv).constants.forM fun _ ci => do
+    if let .inductInfo iv := ci then
+      if !iv.isNested then
+        checkRec iv
+        checkCasesOn iv
+
+partial def mkFreshNames (names : List Name) (count : Nat) (pre := `u) (start := 1) : List Name :=
+  match count with
+  | 0 => []
+  | count + 1 =>
+    let name := pre.appendIndexAfter start
+    if names.contains name then
+      mkFreshNames names (count + 1) pre (start + 1)
+    else
+      name :: mkFreshNames names count pre (start + 1)
+
+def withModifyLocalDecls (xs : Array Expr) (f : LocalDecl → MetaM LocalDecl) (k : MetaM α) : MetaM α := do
+  let ctx ← read
+  let ctx := { ctx with lctx := ← xs.foldlM (init := ctx.lctx) fun lctx x => do
+    let ldecl ← f (lctx.get! x.fvarId!)
+    return lctx.modifyLocalDecl x.fvarId! fun _ => ldecl
+  }
+  withReader (fun _ => ctx) k
+
+def mkRecAux (rv : RecursorVal) : MetaM Unit := do
+  if rv.numMotives == 1 then
+    return
+
+  forallTelescope rv.type fun args ty => do
+  let params := args[:rv.numParams]
+  let motives := args[rv.numParams:rv.numParams+rv.numMotives]
+  let minors := args[rv.numParams+rv.numMotives:rv.numParams+rv.numMotives+rv.numMinors]
+  let indicesMajor := args[rv.numParams+rv.numMotives+rv.numMinors:]
+
+  let .sort u@(.param _) := (← motives[0]!.fvarId!.getType).getForallBody
+    | return
+
+  let levels := mkFreshNames rv.levelParams.tail! rv.numMotives
+  let levelsMap : HashMap FVarId Name := .ofList <| motives.toArray.map (·.fvarId!) |>.toList |>.zip levels
+
+  withModifyLocalDecls motives (fun ldecl => return ldecl.setType <| ldecl.type.replaceLevel (if · == u then some (.param <| levelsMap.find! ldecl.fvarId) else none)) do
+
+  let maxLevel := .mkNaryMax (levels.map .param)
+  let mut e := mkAppN (.const rv.name (.succ maxLevel :: rv.levelParams.tail!.map .param)) params
+
+  for motive in motives do
+    let level := levelsMap.find! motive.fvarId!
+    e := .app e <| ← forallTelescope (← motive.fvarId!.getType) fun args _ =>
+      mkLambdaFVars args <| .app (.const ``ULift [maxLevel, .param level]) (.app (.const ``PLift [.param level]) (mkAppN motive args))
+
+  for minor in minors do
+    e := .app e <| ← forallTelescope (← minor.fvarId!.getType) fun args ty => do
+      let minor := mkAppN minor <| ← args.mapM fun arg => do
+        forallTelescopeReducing (← arg.fvarId!.getType) fun fields type => do
+        let fn := type.getAppFn
+        if fn.isFVar then
+          if let some level := levelsMap.find? fn.fvarId! then
+            let arg := mkAppN arg fields
+            let arg := .app (.app (.const ``ULift.down [maxLevel, .param level]) (.app (.const ``PLift [.param level]) type)) arg
+            let arg := .app (.app (.const ``PLift.down [.param level]) type) arg
+            return ← mkLambdaFVars fields arg
+        return arg
+      withModifyLocalDecls args (fun ldecl => do
+        forallTelescopeReducing ldecl.type fun fields type => do
+        let fn := type.getAppFn
+        if fn.isFVar then
+          if let some level := levelsMap.find? fn.fvarId! then
+            return ldecl.setType <| ← mkForallFVars fields <| .app (.const ``ULift [maxLevel, .param level]) (.app (.const ``PLift [.param level]) type)
+        return ldecl
+      ) do
+      let level := .param <| levelsMap.find! ty.getAppFn.fvarId!
+      let minor := .app (.app (.const ``PLift.up [level]) ty) minor
+      let minor := .app (.app (.const ``ULift.up [maxLevel, level]) (.app (.const ``PLift [level]) ty)) minor
+      mkLambdaFVars args minor
+
+  e := mkAppN e indicesMajor
+
+  let level := .param <| levelsMap.find! ty.getAppFn.fvarId!
+  e := .app (.app (.const ``ULift.down [maxLevel, level]) (.app (.const ``PLift [level]) ty)) e
+  e := .app (.app (.const ``PLift.down [level]) ty) e
+
+  let args := params ++ motives ++ minors ++ indicesMajor
+
+  addDecl <| .defnDecl {
+    name := rv.name.appendAfter "Aux"
+    levelParams := levels ++ rv.levelParams.tail!
+    type := ← mkForallFVars args ty
+    value := ← mkLambdaFVars args e
+    hints := .opaque
+    safety := if rv.isUnsafe then .unsafe else .safe
+  }
+
+run_elab
+  let env ← getEnv
+  env.constants.forM fun _ ci => do
+    let .recInfo rv := ci
+      | return
+    mkRecAux rv
