Common/Structural.lean
@@ -1,0 +1,390 @@
+import Common.Meta
+
+open Lean Parser Meta Elab
+
+elab tk:"@[structural]" fns:Command.mutual : command => withRef tk do
+  let fns ← fns.raw[1].getArgs.mapM fun fn => do Command.mkDefView (← elabModifiers fn[0]) fn[1]
+  if fns.isEmpty then
+    return
+  Command.liftTermElabM do
+  let fns ← _private.Lean.Elab.MutualDef.0.Lean.Elab.Term.elabHeaders fns
+  _private.Lean.Elab.MutualDef.0.Lean.Elab.Term.withFunLocalDecls fns fun fnExprs => do
+
+  let fns ← fns.mapM fun header =>
+    forallBoundedTelescope header.type header.numParams fun defParams type => do
+
+    let .forallE name major body _ ← whnf type
+      | throwErrorAt header.ref "expected function type"
+    let major ← whnf major
+    let some induct := major.getAppFn.constName?
+      | throwErrorAt header.ref "expected inductive type"
+
+    let induct ← getConstInfoInduct induct
+    let args := major.getAppArgs
+    let params := args[:induct.numParams]
+    let indices := args[induct.numParams:]
+
+    let skip := params.foldl collectFVars {} |>.fvarSet
+
+    let (fixedParams, fixedParamsIdx) := defParams.zipWithIndex.filter (skip.contains ·.fst.fvarId!) |>.unzip
+
+    let (skip, indicesIdx) ← indices.foldlM (init := (skip, @Array.mkEmpty Nat indices.size)) fun (skip, indicesIdx) index => do
+      if !index.isFVar then
+        throwErrorAt header.ref "index is not a variable"
+      if skip.contains index.fvarId! then
+        throwErrorAt header.ref "duplicate index variable"
+      return (skip.insert index.fvarId!, indicesIdx.push (defParams.indexOf? index |>.map (↑·)).get!)
+
+    let (genParams, genParamsIdx) := defParams.zipWithIndex.filter (!skip.contains ·.fst.fvarId!) |>.unzip
+
+    let motive ← mkForallFVars genParams <| body.instantiate1 (.bvar genParams.size)
+    let level := (← inferType motive).sortLevel!
+    let motive ← mkForallFVars fixedParams <| ← mkLambdaFVars indices <| .lam name major motive .default
+    return (header, induct, major.getAppFn.constLevels!, motive, level, fixedParamsIdx, indicesIdx, genParamsIdx)
+
+  let (header, induct, levels, motive, level, fixedParamsIdx, _) := fns[0]!
+  forallBoundedTelescope motive fixedParamsIdx.size fun fixedParams _ => do
+  let paramsTy ← mkForallFVars fixedParams <| .const ``Unit []
+
+  let recLevels ← do
+    if (← getConstInfoRec (mkRecName induct.name)).levelParams.length > induct.levelParams.length then
+      pure <| level :: levels
+    else
+      if level != .zero then
+        throwErrorAt header.ref m!"cannot eliminate into non-prop sort"
+      pure levels
+
+  for (header', _, levels', motive', level', fixedParamsIdx', _) in fns[1:] do
+    if header'.levelNames != header.levelNames then
+      throwErrorAt header'.ref m!"different level parameters"
+    if levels' != levels then
+      throwErrorAt header'.ref m!"levels mismatch"
+    if level' != level then
+      throwErrorAt header'.ref m!"output sort mismatch"
+    forallBoundedTelescope motive' fixedParamsIdx'.size fun fixedParams' _ => do
+      let paramsTy' ← mkForallFVars fixedParams' <| .const ``Unit []
+      if !(← isDefEq paramsTy paramsTy') then
+        throwErrorAt header'.ref m!"fixed params differ"
+
+  let fns ← fns.mapM fun (header, induct, _, motive, _, fixedParamsIdx, indicesIdx, genParamsIdx) =>
+    Elab.Term.withDeclName header.declName do
+
+    let `(Command.declValEqns| $alts:matchAlt*) := header.valueStx
+      | throwErrorAt header.valueStx "expected match arms"
+    let alts ← liftMacroM <| alts.concatMapM Term.expandMatchAlt
+    let alts ← alts.mapM fun alt => do
+      match alt with
+      | `(Term.matchAltExpr| | $pattern => $rhs) =>
+        return {
+          ref := alt
+          patterns := #[pattern]
+          rhs
+        }
+      | _ => throwErrorAt alt "expected match arm with single pattern"
+    let alts ← liftMacroM <| Term.expandMacrosInPatterns alts
+
+    let motive' ← instantiateForall motive fixedParams
+
+    let motives ← fns.foldlM (init := mkHashMap) fun motives (_, induct, _, motive, _) =>
+      return motives.insert induct.name <| ← instantiateForall motive fixedParams
+
+    let alts ← alts.mapM fun alt => do
+      let (pVars, alt) ← Term.collectPatternVars alt
+      _private.Lean.Elab.Match.0.Lean.Elab.Term.withPatternVars pVars fun pVarDecls => do
+      let (_, _, .lam _ major motive _) ← lambdaMetaTelescope motive' induct.numIndices
+        | unreachable!
+
+      let lhs ← Term.elabTermEnsuringType alt.patterns[0]! major
+      let lhs ← instantiateMVars lhs
+
+      let mvars := lhs.collectMVars {} |>.result
+      let extraFields ← mvars.mapM fun mvar => do
+        let decl ← mvar.getDecl
+        return (decl.userName, fun _ => return decl.type)
+      withLocalDeclsD extraFields fun extraFields => do
+      modifyMCtx fun mctx => { mctx with eAssignment := mvars.zip extraFields |>.foldl (init := mctx.eAssignment) fun eAssignment (mvar, fvar) => eAssignment.insert mvar fvar }
+
+      let lhs ← instantiateMVars lhs
+      let lhs ← whnf lhs
+
+      let some ctor := lhs.getAppFn.constName?
+        | throwErrorAt alt.patterns[0]! "not a constructor"
+      let cv ← getConstInfoCtor ctor
+      let fields := lhs.getAppArgs[cv.numParams:].toArray
+      for field in fields do
+        if !field.isFVar || (!pVarDecls.any (·.fvarId == field.fvarId!) && !extraFields.any (· == field)) then
+          throwErrorAt alt.patterns[0]! "field is not a variable"
+
+      let (ihFields, ihs) := Array.unzip <| ← fields.filterMapM fun field => do
+        forallTelescopeReducing (← instantiateMVars <| ← field.fvarId!.getType) fun xs t => do
+          t.getAppFn.constName?.bindM fun fn => do
+          motives.find? fn |>.mapM fun motive => do
+          let ih ← mkForallFVars xs <| ← instantiateLambda motive <| t.getAppArgs[induct.numParams:].toArray.push (mkAppN field xs)
+          return (field, (← field.fvarId!.getUserName).appendAfter "_ih", (fun _ => return ih : Array _ → TermElabM _))
+      withLocalDeclsD ihs fun ihs =>
+
+      forallBoundedTelescope (motive.instantiate1 lhs) genParamsIdx.size fun genParams body => do
+      let rhs ← Term.elabTermEnsuringType alt.rhs body
+      Term.synthesizeSyntheticMVars
+      let rhs ← instantiateMVars rhs
+
+      let minor ← transform rhs (post := fun e => do
+        let some stx := getRecAppSyntax? e
+          | return .done e
+        let args := e.mdataExpr!.getAppArgs
+        if args.size <= header.numParams then
+          throwErrorAt stx "not enough arguments"
+        if fixedParamsIdx.map args.get! != fixedParams then
+          throwErrorAt stx "fixed params difer"
+        let major := args[header.numParams]!
+        let some idx := ihFields.indexOf? major.getAppFn
+          | throwErrorAt stx "invalid recursive call"
+        return .done <| mkAppN (mkAppN (mkAppN ihs[idx]! major.getAppArgs) (genParamsIdx.map args.get!)) args[header.numParams + 1:]
+      )
+
+      let rhs ← transform rhs (post := fun e => do
+        if !e.isMData then
+          return .done e
+        let some idx := fnExprs.indexOf? e.mdataExpr!.getAppFn
+          | return .done e
+        return .done <| mkAppN (.const fns[idx]!.fst.declName (header.levelNames.map .param)) e.mdataExpr!.getAppArgs
+      )
+
+      return (alt.patterns[0]!, cv.name, ← mkLambdaFVars (fixedParams ++ fields ++ genParams) rhs, ← mkLambdaFVars (fixedParams ++ fields ++ ihs ++ genParams) minor)
+
+    let alts ← alts.foldlM (init := mkHashMap) fun alts (ref, ctor, alt) =>
+      if alts.contains ctor then
+        throwErrorAt ref "duplicate constructor"
+      else
+        return alts.insert ctor alt
+
+    let alts ← induct.ctors.mapM fun ctor =>
+      if let some alt := alts.find? ctor then
+        return alt
+      else
+        throwErrorAt header.ref m!"missing constructor: {ctor}"
+
+    return (header, induct, motive, alts, fixedParamsIdx, indicesIdx, genParamsIdx)
+
+  let fns ← fns.foldlM (init := mkHashMap) fun fns (header, induct, fn) =>
+    if fns.contains induct.name then
+      throwErrorAt header.ref "duplicate inductive"
+    else
+      return fns.insert induct.name (header, induct, fn)
+
+  let fns ← induct.all.toArray.mapM fun induct =>
+    if let some fn := fns.find? induct then
+      return fn
+    else
+      throwError "missing inductive: {induct}"
+
+  for (header, _, _, _, fixedParamsIdx, indicesIdx, genParamsIdx) in fns do
+    forallBoundedTelescope header.type (some (header.numParams + 1)) fun defParams _ => do
+    let fixedParams := fixedParamsIdx.map defParams.get!
+    let indices := indicesIdx.map defParams.get!
+    let genParams := genParamsIdx.map defParams.get!
+
+    let major := defParams.back
+    let majorTy ← major.fvarId!.getType
+    let majorTy ← whnf majorTy
+    let induct := majorTy.getAppFn
+    let args := majorTy.getAppArgs
+
+    let mut e := .const (mkRecName induct.constName!) recLevels
+    e := mkAppN e args[:args.size - indices.size]
+    e := mkAppN e <| ← fns.mapM fun (_, _, motive, _) => instantiateForall motive fixedParams
+    e := mkAppN e <| ← fns.concatMapM fun (_, _, _, alts, _) => alts.toArray.mapM fun (_, minor) => instantiateLambda minor fixedParams
+    e := mkAppN e indices
+    e := .app e major
+    e := mkAppN e genParams
+
+    addDecl <| .defnDecl {
+      name := header.declName
+      levelParams := header.levelNames
+      type := header.type
+      value := ← mkLambdaFVars defParams e
+      hints := .opaque
+      safety := if header.modifiers.isUnsafe then .unsafe else .safe
+    }
+
+  for (header, induct, motive, alts, fixedParamsIdx, indicesIdx, genParamsIdx) in fns do
+    forallBoundedTelescope header.type (some (header.numParams + 1)) fun defParams _ => do
+    let fixedParams := fixedParamsIdx.map defParams.get!
+    let indices := indicesIdx.map defParams.get!
+    let genParams := genParamsIdx.map defParams.get!
+
+    let major := defParams.back
+    let majorTy ← major.fvarId!.getType
+    let majorTy ← whnf majorTy
+    let args := majorTy.getAppArgs
+
+    let casesOn := mkCasesOnName induct.name
+
+    let mut e := .const casesOn recLevels
+    e := mkAppN e args[:args.size - indices.size]
+    e := .app e <| ← instantiateForall motive fixedParams
+    e := mkAppN e indices
+    e := .app e major
+    e := mkAppN e <| ← alts.toArray.mapM fun (rhs, _) => instantiateLambda rhs fixedParams
+    e := mkAppN e genParams
+
+    addDecl <| .defnDecl {
+      name := Compiler.mkUnsafeRecName header.declName
+      levelParams := header.levelNames
+      type := header.type
+      value := ← mkLambdaFVars defParams e
+      hints := .opaque
+      safety := if header.modifiers.isUnsafe then .unsafe else .safe
+    }
+
+    let matcherName ← mkAuxName (header.declName.str "match") 1
+    let casesOnInfo ← getConstInfo casesOn
+
+    addDecl <| .defnDecl {
+      name := matcherName
+      levelParams := casesOnInfo.levelParams
+      type := casesOnInfo.type
+      value := .const casesOn (casesOnInfo.levelParams.map .param)
+      hints := .abbrev
+      safety := .safe
+    }
+
+    Match.addMatcherInfo matcherName {
+        numParams := induct.numParams
+        numDiscrs := induct.numIndices + 1
+        altNumParams := ← induct.ctors.toArray.mapM fun ctor => return (← getConstInfoCtor ctor).numFields
+        uElimPos? := if casesOnInfo.levelParams.length == levels.length then none else some 0
+        discrInfos := #[]
+    }
+
+    e := .const matcherName recLevels
+    e := mkAppN e args[:args.size - indices.size]
+    e := .app e <| ← instantiateForall motive fixedParams
+    e := mkAppN e indices
+    e := .app e major
+    e := mkAppN e <| ← alts.toArray.mapM fun (rhs, _) => do
+      let rhs ← instantiateLambda rhs fixedParams
+      lambdaTelescope rhs fun xs rhs => do
+        mkLambdaFVars xs[:xs.size - genParams.size] <| markSmartUnfoldingMatchAlt <| ← mkLambdaFVars xs[xs.size - genParams.size:] rhs
+    e := markSmartUnfoldingMatch e
+    e := mkAppN e genParams
+
+    addDecl <| .defnDecl {
+      name := mkSmartUnfoldingNameFor header.declName
+      levelParams := header.levelNames
+      type := header.type
+      value := ← mkLambdaFVars defParams e
+      hints := .opaque
+      safety := if header.modifiers.isUnsafe then .unsafe else .safe
+    }
+
+  compileDecls <| Array.toList <| fns.map fun (header, _) => Compiler.mkUnsafeRecName header.declName
+
+  -- TODO equations
+  -- TODO eq_def
+
+  for (header, _) in fns do
+    Term.applyAttributes header.declName header.modifiers.attrs
+
+/-
+mutual
+
+inductive Even
+  | zero
+  | succ (o : Odd)
+
+inductive Odd
+  | succ (e : Even)
+
+end
+
+@[structural]
+mutual
+
+def Odd.toNat : (o : Odd) → Nat
+  | .succ e => .succ e.toNat
+
+def Even.toNat : (e : Even) → Nat
+  | .succ o => .succ o.toNat
+  | .zero   => .zero
+
+end
+
+@[structural]
+mutual
+
+def List.id {α : Type u} : List α → List α
+  | [] => []
+  | x :: xs => x :: xs.id
+
+end
+
+@[structural]
+mutual
+
+def List.mem {α : Type u} : (l : List α) → List { x // x ∈ l }
+  | [] => []
+  | x :: xs => ⟨x, .head xs⟩ :: xs.mem.map fun ⟨_, h⟩ => ⟨_, .tail x h⟩
+
+end
+
+inductive Fin2 : Nat → Type
+  | zero : Fin2 (.succ n)
+  | succ : Fin2 n → Fin2 n.succ
+
+@[structural]
+mutual
+
+def Fin2.toNat : Fin2 n → Nat
+  | .zero   => .zero
+  | .succ i => .succ i.toNat
+
+end
+
+inductive Ordinal
+  | zero
+  | succ (o : Ordinal)
+  | limit (os : Nat → Ordinal)
+
+@[structural]
+mutual
+
+def Ordinal.add (x : Ordinal) : (y : Ordinal) → Ordinal
+  | .zero => x
+  | .succ y => .succ (x.add y)
+  | .limit ys => .limit (x.add <| ys ·)
+
+end
+
+@[structural]
+mutual
+
+def List_id {α : Sort u} : List (PLift α) → List (PLift α)
+  | [] => []
+  | x :: xs => x :: xs
+
+end
+
+mutual
+
+inductive EvenList (α : Type u)
+  | nil
+  | cons (x : α) (xs : OddList α)
+
+inductive OddList (α : Type u)
+  | cons (x : α) (xs : EvenList α)
+
+end
+
+@[structural]
+mutual
+
+def EvenList.toList {α : Type u} : EvenList α → List α
+  | .nil       => .nil
+  | .cons x xs => .cons x xs.toList
+
+def OddList.toList {α : Type u} : OddList α → List α
+  | .cons x xs => .cons x xs.toList
+
+end
+-/
