lakefile.lean
@@ -1,9 +1,0 @@
-import Lake
-open Lake DSL
-
-package «lean-stuff»
-
-lean_lib Common
-lean_lib STLC
-
-require mathlib from git "https://github.com/leanprover-community/mathlib4.git"
